isabelle/Testing.thy
@@ -22,11 +22,10 @@ definition test_post_parse :: "string \<Rightarrow> (Location \<times> PostParse
 
 (* value "lex ''Test.b'' ''0x10000000000000000''" *)
 
+value "test_parser parse_term ''y.x<i32>''"
 
 value "test_parser parse_module ''module Main
 interface {}
+  const c = match 1 { case (2) => 3 };
 
-function foo(): i32
-{
-    return (match 1 { case 2 => 3; case 3 => 0 });
-}''"
+''"
